src/Language/PlutusIR/Semantics/SemanticEquivalence/CompatibilityLemmas/DatatypeBind.v
@@ -2,15 +2,118 @@ Require Import PlutusCert.Language.PlutusIR.Semantics.Dynamic.
 Require Import PlutusCert.Language.PlutusIR.Semantics.Static.
 Require Import PlutusCert.Language.PlutusIR.Semantics.SemanticEquivalence.LogicalRelation.
 Require Import PlutusCert.Language.PlutusIR.Semantics.SemanticEquivalence.Auto.
+Require Import PlutusCert.Language.PlutusIR.Semantics.SemanticEquivalence.Multisubstitution.Congruence.
+
+Require Import Coq.Lists.List.
 
 
 
-Lemma compatibility_DatatypeBind : forall Delta Gamma d,
-    Delta ,, Gamma |-ok_b (DatatypeBind d) ->
-    LR_logically_approximate_binding Delta Gamma (DatatypeBind d) (DatatypeBind d).
-Proof with eauto_LR.
-  intros Delta Gamma d Hok.
-  unfold LR_logically_approximate_binding.
-
-  split...
+Lemma msubst_DatatypeBind : forall ss X YKs matchFunc cs,
+    msubst_binding ss (DatatypeBind (Datatype X YKs matchFunc cs)) = DatatypeBind (Datatype X YKs matchFunc cs).
+Proof.
+  induction ss; intros.
+  - reflexivity.
+  - destruct a. eauto.
 Qed.
+
+Lemma msubstA_DatatypeBind : forall ss X YKs matchFunc cs,
+    msubstA_binding ss (DatatypeBind (Datatype X YKs matchFunc cs)) = DatatypeBind (Datatype X YKs matchFunc (msubstA_constructors ss cs)).
+Proof.
+  induction ss; intros.
+  - reflexivity.
+  - destruct a. simpl. eauto.
+Qed.
+
+
+Lemma mupdate_flatten : forall {X : Type} (m : partial_map X) x l,
+    mupdate m (flatten (x :: l)) = mupdate (mupdate m x) (flatten l).
+Proof.
+  intros.
+  unfold flatten.
+  simpl.
+  rewrite List.concat_app.
+  simpl.
+  rewrite List.app_nil_r.
+  rewrite <- mupdate_app.
+  reflexivity.
+Qed.
+
+Lemma map_normalise__app' : forall l1 l1n l2 l2n,
+    map_normalise l1 l1n ->
+    map_normalise l2 l2n ->
+    map_normalise (l1 ++ l2) (l1n ++ l2n).
+Proof.
+  induction l1; intros.
+  - inversion H. subst. simpl. eauto.
+  - inversion H. subst. simpl. econstructor. eauto. eauto.
+Qed.
+
+
+Lemma compatibility_DatatypeBind : forall Delta Gamma X YKs cs matchFunc Delta' b b' bs bs' t t' Tn,
+    Delta' = mupdate Delta (rev (map fromDecl YKs)) ->
+    (forall c, In c cs -> Delta' |-ok_c c : (constrLastTy (Datatype X YKs matchFunc cs))) ->
+    forall Delta_ih Gamma_ih bsGn,
+      b = DatatypeBind (Datatype X YKs matchFunc cs) ->
+      b' = DatatypeBind (Datatype X YKs matchFunc cs) ->
+      Delta_ih = mupdate Delta (binds_Delta b) ->
+      map_normalise (binds_Gamma b) bsGn ->
+      Gamma_ih = mupdate Gamma bsGn ->
+      LR_logically_approximate Delta_ih Gamma_ih (Let NonRec bs t) (Let NonRec bs' t') Tn ->
+      LR_logically_approximate Delta Gamma (Let NonRec (b :: bs) t) (Let NonRec (b' :: bs') t') Tn.
+Proof with eauto_LR.
+  intros Delta Gamma X YKs cs matchFunc Delta' b b' bs bs' t t' Tn.
+  intros Heq__Delta' Hok__cs.
+  intros Delta_ih Gamma_ih bsGn.
+  intros Heq__b Heq__b' Heq__Delta_ih Hmapnorm__bsGn Heq__Gamma_ih IHLR__ih.
+
+  subst.
+
+  destruct IHLR__ih as [Htyp__ih [Htyp__ih' IH__ih]].
+
+  split. {
+    inversion Htyp__ih. subst.
+    rewrite <- mupdate_flatten in H7.
+
+    eapply T_Let...
+    - unfold flatten.
+      simpl.
+      simpl in Hmapnorm__bsGn.
+      rewrite List.concat_app.
+      eapply map_normalise__app'...
+      admit.
+    - rewrite mupdate_app. eapply H7.
+    - admit. 
+  }
+
+  split. {
+    inversion Htyp__ih'. subst.
+    rewrite <- mupdate_flatten in H7.
+
+    eapply T_Let...
+    - unfold flatten.
+      simpl.
+      simpl in Hmapnorm__bsGn.
+      rewrite List.concat_app.
+      eapply map_normalise__app'...
+      admit.
+    - rewrite mupdate_app. eapply H7.
+    - admit.
+  }
+
+  intros k rho env env' ct ck HeqDelta HeqGamma HRD HRG.
+  subst.
+
+  rewrite msubstA_LetNonRec.
+  rewrite msubstA_BindingsNonRec_cons.
+  rewrite msubstA_DatatypeBind.
+  rewrite msubst_LetNonRec.
+  rewrite msubst_BindingsNonRec_cons.
+  rewrite msubst_DatatypeBind.
+
+  autorewrite with RC.
+
+  intros j Hlt__j e_f Hev__e_f.
+  inversion Hev__e_f. subst.
+  clear Hev__e_f. rename H3 into Hev__e_f.
+  inversion Hev__e_f; subst.
+Admitted.
