src/Language/PlutusIR/Semantics/SemanticEquivalence/CompatibilityLemmas/TermBind.v
@@ -2,6 +2,14 @@ Require Import PlutusCert.Language.PlutusIR.Semantics.Dynamic.
 Require Import PlutusCert.Language.PlutusIR.Semantics.Static.
 Require Import PlutusCert.Language.PlutusIR.Semantics.SemanticEquivalence.LogicalRelation.
 Require Import PlutusCert.Language.PlutusIR.Semantics.SemanticEquivalence.Auto.
+Require Import PlutusCert.Language.PlutusIR.Semantics.SemanticEquivalence.Multisubstitution.Congruence.
+
+Require Import PlutusCert.Util.
+
+Require Import Coq.Lists.List.
+
+Local Open Scope list_scope.
+
 
 
 Lemma msubst_TermBind : forall ss stricty x T e,
@@ -20,22 +28,332 @@ Proof.
   - destruct a. eauto.
 Qed.
 
-Lemma compatibility_TermBind : forall Delta Gamma stricty x T t t',
-    Delta |-* T : Kind_Base ->
-    LR_logically_approximate Delta Gamma t t' T ->
-    LR_logically_approximate_binding Delta Gamma (TermBind stricty (VarDecl x T) t) (TermBind stricty (VarDecl x T) t').
-Proof with eauto_LR.
-  intros Delta Gamma stricty X T t t' Hkind__T IH_LR.
-  unfold LR_logically_approximate_binding.
-
-  destruct IH_LR as [Htyp__t [Htyp__t' IH__t]].
-
-  split...
-  split...
-
-  split...
-  split...
-  split...
-  
-  split...
+Lemma mupdate_flatten : forall {X : Type} (m : partial_map X) x l,
+    mupdate m (flatten (x :: l)) = mupdate (mupdate m x) (flatten l).
+Proof.
+  intros.
+  unfold flatten.
+  simpl.
+  rewrite List.concat_app.
+  simpl.
+  rewrite List.app_nil_r.
+  rewrite <- mupdate_app.
+  reflexivity.
 Qed.
+
+Lemma map_normalise__app' : forall l1 l1n l2 l2n,
+    map_normalise l1 l1n ->
+    map_normalise l2 l2n ->
+    map_normalise (l1 ++ l2) (l1n ++ l2n).
+Proof.
+  induction l1; intros.
+  - inversion H. subst. simpl. eauto.
+  - inversion H. subst. simpl. econstructor. eauto. eauto.
+Qed.
+
+
+Lemma compatibility_TermBind : forall Delta Gamma stricty x Tb Tbn tb tb' b b' bs bs' t t' Tn,
+    Delta |-* Tb : Kind_Base ->
+    normalise Tb Tbn ->
+    forall Delta_ih Gamma_ih bsGn,
+      b = TermBind stricty (VarDecl x Tb) tb ->
+      b' = TermBind stricty (VarDecl x Tb) tb' ->
+      Delta_ih = mupdate Delta (binds_Delta b) ->
+      map_normalise (binds_Gamma b) bsGn ->
+      Gamma_ih = mupdate Gamma bsGn ->
+      LR_logically_approximate Delta_ih Gamma_ih (Let NonRec bs t) (Let NonRec bs' t') Tn ->
+      LR_logically_approximate Delta Gamma tb tb' Tbn ->
+      LR_logically_approximate Delta Gamma (Let NonRec (b :: bs) t) (Let NonRec (b' :: bs') t') Tn.
+Proof with eauto_LR.
+  intros Delta Gamma stricty x Tb Tbn tb tb' b b' bs bs' t t' Tn.
+  intros Hkind__Tb Hnorm__Tbn.
+  intros Delta_ih Gamma_ih bsGn.
+  intros Heq__b Heq__b' Heq__Delta_ih Hmapnorm__bsGn Heq__Gamma_ih IHLR__ih IHLR__tb.
+
+  subst.
+
+  destruct IHLR__ih as [Htyp__ih [Htyp__ih' IH__ih]].
+  destruct IHLR__tb as [Htyp__tb [Htyp__tb' IH__tb]].
+
+  split. {
+    inversion Htyp__ih. subst.
+    rewrite <- mupdate_flatten in H7.
+
+    eapply T_Let...
+    - unfold flatten.
+      simpl.
+      simpl in Hmapnorm__bsGn.
+      rewrite List.concat_app.
+      eapply map_normalise__app'...
+    - rewrite mupdate_app. eapply H7.
+  }
+
+  split. {
+    inversion Htyp__ih'. subst.
+    rewrite <- mupdate_flatten in H7.
+
+    eapply T_Let...
+    - unfold flatten.
+      simpl.
+      simpl in Hmapnorm__bsGn.
+      rewrite List.concat_app.
+      eapply map_normalise__app'...
+    - rewrite mupdate_app. eapply H7.
+  }
+
+  intros k rho env env' ct ck HeqDelta HeqGamma HRD HRG.
+  subst.
+  
+  rewrite msubstA_LetNonRec.
+  rewrite msubstA_BindingsNonRec_cons.
+  rewrite msubstA_TermBind.
+  rewrite msubst_LetNonRec.
+  rewrite msubst_BindingsNonRec_cons.
+  rewrite msubst_TermBind.
+
+  autorewrite with RC.
+
+  intros j Hlt__j e_f Hev__e_f.
+  inversion Hev__e_f. subst.
+  clear Hev__e_f. rename H3 into Hev__e_f.
+  inversion Hev__e_f; subst.
+  - (* E_Let_TermBind *)
+    clear Hev__e_f.
+    rename v1 into vb.
+    rename j1 into jb.
+    rename H7 into Hev__vb.
+    rename H9 into Hev__e_f.
+
+    assert (HRC__tb :
+    RC k Tbn rho
+      (msubst_term env (msubstA_term (msyn1 rho) tb))
+      (msubst_term env' (msubstA_term (msyn2 rho) tb'))  
+    )...
+    clear IH__tb.
+
+    eapply RC_to_RV with (j := jb) (e_f := vb) in HRC__tb as temp...
+    destruct temp as [vb' [jb' [Hev__vb' HRV__vb]]].
+    clear Hev__vb.
+    clear HRC__tb.
+  
+    assert (HRC__ih :
+      RC (k - jb - 1) Tn rho
+        <{ /[ (x, vb) :: drop x env /] ( /[[ msyn1 rho /] {Let NonRec bs t} ) }>
+        <{ /[ (x, vb') :: drop x env' /] ( /[[ msyn2 rho /] {Let NonRec bs' t'} ) }>
+    ). {
+      apply IH__ih with (ct0 := (x, Tbn) :: drop x ct) (ck0 := ck).
+      - reflexivity.
+      - inversion Hmapnorm__bsGn. subst.
+        inversion H3. subst.
+        simpl.
+        eapply normalisation__deterministic in Hnorm__Tbn...
+        subst.
+        apply mupdate_drop.
+      - assumption.
+      - assert (closed vb). {
+          eapply RV_typable_empty_1 in HRV__vb...
+          destruct HRV__vb as [Tbn' [_ Htyp]].
+          eapply typable_empty__closed...
+        }
+        assert (closed vb'). {
+          eapply RV_typable_empty_2 in HRV__vb...
+          destruct HRV__vb as [Tbn' [_ Htyp]].
+          eapply typable_empty__closed...
+        }
+        replace vb with (msubstA_term (msyn1 rho) vb) by (eapply msubstA_closed; eauto).
+        replace vb' with (msubstA_term (msyn2 rho) vb') by (eapply msubstA_closed; eauto).
+        apply RG_cons.
+        + apply RV_monotone with (k := k - jb) (ck := ck)...
+          rewrite msubstA_closed...
+          rewrite msubstA_closed...
+        + eapply normalise_to_normal...
+        + apply RG_monotone with (k := k) (ck := ck)...
+          apply RG_drop...
+    }
+    clear IH__ih.
+
+    apply RC_to_RV with (j := j2) (e_f := e_f) in HRC__ih as temp...
+    + destruct temp as [e'_f [j0' [Hev__e'_f HRV0]]].
+      clear Hev__e_f.
+
+      rewrite msubstA_LetNonRec.
+      rewrite msubstA_BindingsNonRec_cons.
+      rewrite msubstA_TermBind.
+      rewrite msubst_LetNonRec.
+      rewrite msubst_BindingsNonRec_cons.
+      rewrite msubst_TermBind.
+    
+      rewrite msubstA_LetNonRec in Hev__e'_f.
+      rewrite msubst_LetNonRec in Hev__e'_f.
+
+      rewrite <- msubstA_bnr__bvbs in Hev__e'_f.
+
+      inversion Hev__e'_f. subst.
+
+      eexists. eexists.
+      split. {
+        apply E_Let.
+        apply E_Let_TermBind with (v1 := vb') (j1 := jb') (v2 := e'_f) (j2 := j0')...
+        1: {
+          eapply RV_error in HRV__vb...
+          destruct HRV__vb as [ [Hnerr Hnerr'] | [Herr Herr']]...
+        }
+        simpl.
+        rewrite <- msubst_bnr__bound_vars.
+        rewrite <- msubstA_bnr__bvbs.
+        destruct (existsb (eqb x) (bvbs bs')) eqn:Hexb.
+        - assert (closed vb). eapply RV_closed_1...
+          assert (closed vb'). eapply RV_closed_2...
+          apply RG_env_closed in HRG as Hclss...
+          destruct Hclss as [Hcls__env Hcls__env'].
+          rewrite <- subst_bnr__msubst_bnr'...
+          replace (concat (map bvb <{ /[[ msyn2 rho /][bnr] bs' }>)) with
+            (bvbs  <{ /[[ msyn2 rho /][bnr] bs' }>)...
+          rewrite <- msubstA_bnr__bvbs.
+
+          apply existsb_exists in Hexb.
+          destruct Hexb as [y [HIn Heqb]].
+          apply eqb_eq in Heqb as Heq.
+          subst.
+          rewrite In__mdrop in H3...
+        - assert (closed vb). eapply RV_closed_1...
+          assert (closed vb'). eapply RV_closed_2...
+          apply RG_env_closed in HRG as Hclss...
+          destruct Hclss as [Hcls__env Hcls__env'].
+          rewrite <- subst_bnr__msubst_bnr'...
+          replace (concat (map bvb <{ /[[ msyn2 rho /][bnr] bs' }>)) with
+            (bvbs  <{ /[[ msyn2 rho /][bnr] bs' }>)...
+          rewrite <- msubstA_bnr__bvbs.
+
+          apply existsb_nexists in Hexb.
+          rewrite not_In__mdrop in H3...
+          + unfold btvbs. simpl.
+            replace (concat (map btvb bs')) with (btvbs bs')...
+
+            rewrite <- subst_msubst''...
+            * eapply RG_env_closed.
+              eapply RG_drop...
+              eauto_LR.
+            * intros Hcon.
+              apply Hexb.
+              exists x.
+              rewrite eqb_refl.
+              eauto.
+          + intros Hcon.
+            apply Hexb.
+            exists x.
+            rewrite eqb_refl.
+            eauto.
+      }
+
+      split... eapply RV_typable_empty_1...
+      split... eapply RV_typable_empty_2...
+    
+      eapply RV_condition...
+      eapply RV_monotone...
+
+    + rewrite msubstA_LetNonRec.
+      rewrite msubst_LetNonRec. 
+      apply E_Let.
+
+      simpl.
+      simpl in Hev__e_f.
+
+      rewrite <- msubst_bnr__bound_vars in Hev__e_f.
+      rewrite <- msubstA_bnr__bvbs in Hev__e_f.
+
+      destruct (existsb (eqb x) (bvbs bs)) eqn:Hexb. {
+        assert (closed vb). eapply RV_closed_1...
+        assert (closed vb'). eapply RV_closed_2...
+        apply RG_env_closed in HRG as Hclss...
+        destruct Hclss as [Hcls__env Hcls__env'].
+        rewrite <- subst_bnr__msubst_bnr' in Hev__e_f...
+        replace (concat (map bvb <{ /[[ msyn1 rho /][bnr] bs }>)) with
+          (bvbs <{ /[[ msyn1 rho /][bnr] bs }>) in Hev__e_f...
+        
+        unfold btvbs in Hev__e_f.
+        simpl in Hev__e_f.
+        rewrite <- msubstA_bnr__bvbs.
+        rewrite <- msubstA_bnr__bvbs in Hev__e_f.
+
+        apply existsb_exists in Hexb.
+        destruct Hexb as [y [HIn Heqb]].
+        apply eqb_eq in Heqb as Heq.
+        subst.
+        rewrite In__mdrop...
+      } {
+        assert (closed vb). eapply RV_closed_1...
+        assert (closed vb'). eapply RV_closed_2...
+        apply RG_env_closed in HRG as Hclss...
+        destruct Hclss as [Hcls__env Hcls__env'].
+        rewrite <- subst_bnr__msubst_bnr' in Hev__e_f...
+        replace (concat (map bvb <{ /[[ msyn1 rho /][bnr] bs }>)) with
+          (bvbs <{ /[[ msyn1 rho /][bnr] bs }>) in Hev__e_f...
+        
+        unfold btvbs in Hev__e_f.
+        simpl in Hev__e_f.
+        rewrite <- msubstA_bnr__bvbs.
+        rewrite <- msubstA_bnr__bvbs in Hev__e_f.
+
+        apply Util.existsb_nexists in Hexb.
+        rewrite not_In__mdrop.
+        - replace (concat (map btvb bs)) with (btvbs bs) in Hev__e_f...
+          rewrite <- subst_msubst'' in Hev__e_f...
+          + eapply RG_env_closed_1.
+            eapply RG_drop...
+            eauto_LR.
+          + intros Hcon.
+            apply Hexb.
+            exists x.
+            rewrite eqb_refl.
+            eauto.
+        - intros Hcon.
+          apply Hexb.
+          exists x.
+          rewrite eqb_refl.
+          eauto.
+      }
+  - (* E_Error_Let_TermBind*)
+    rename j1 into jb.
+    rename H7 into Hev__Err.
+
+    assert (HRC__tb :
+      RC k Tbn rho
+        (msubst_term env (msubstA_term (msyn1 rho) tb))
+        (msubst_term env' (msubstA_term (msyn2 rho) tb'))  
+      )...
+    clear IH__tb.
+
+    eapply RC_to_RV with (j := jb) (e_f := Error T') in HRC__tb as temp...
+    destruct temp as [vb' [jb' [Hev__vb' HRV__vb]]].
+    clear Hev__Err.
+    clear HRC__tb.
+
+    eapply RV_error in HRV__vb as temp...
+    
+    destruct temp as [ [Hnerr Hnerr'] | [Herr Herr']].
+    + exfalso. eapply Hnerr. econstructor.
+    + inversion Herr'. subst.
+
+      eexists. eexists.
+      split. {
+        rewrite msubstA_LetNonRec.
+        rewrite msubstA_BindingsNonRec_cons.
+        rewrite msubstA_TermBind.
+        rewrite msubst_LetNonRec.
+        rewrite msubst_BindingsNonRec_cons.
+        rewrite msubst_TermBind.
+
+        eapply E_Let.
+        eapply E_Error_Let_TermBind...
+      }
+      
+      split. {
+        admit.
+      }
+
+      split. {
+        admit.
+      }
+      right...
+Admitted.
