src/Language/PlutusIR/Semantics/SemanticEquivalence/FundamentalProperty.v
@@ -1,25 +1,31 @@
 Require Import PlutusCert.Language.PlutusIR.Semantics.Dynamic.
 Require Import PlutusCert.Language.PlutusIR.Semantics.Static.
 Require Import PlutusCert.Language.PlutusIR.Semantics.SemanticEquivalence.CompatibilityLemmas.
-Require Import PlutusCert.Language.PlutusIR.Semantics.SemanticEquivalence.LogicalRelation.RelationalModel.
+Require Import PlutusCert.Language.PlutusIR.Semantics.SemanticEquivalence.LogicalRelation.
 
 
 Definition P_has_type Delta Gamma e T := 
   LR_logically_approximate Delta Gamma e e T.
 
-Definition P_constructor_well_formed Delta c := Delta |-ok_c c.
+Definition P_constructor_well_formed Delta c Tr := Delta |-ok_c c : Tr.
 
 Definition P_bindings_well_formed_nonrec Delta Gamma (bs : list Binding) := 
-  forall Delta_t Gamma_t t t' T,
+  forall Delta_t Gamma_t bsGn t t' T,
     Delta_t = mupdate Delta (flatten (List.map binds_Delta bs)) ->
-    Gamma_t = mupdate Gamma (flatten (List.map binds_Gamma bs)) ->
+    map_normalise (flatten (List.map binds_Gamma bs)) bsGn ->
+    Gamma_t = mupdate Gamma bsGn  ->
     LR_logically_approximate Delta_t Gamma_t t t' T ->
     LR_logically_approximate Delta Gamma (Let NonRec bs t) (Let NonRec bs t') T.
 
 Definition P_bindings_well_formed_rec Delta Gamma bs1 := Delta ,, Gamma |-oks_r bs1.
 
 Definition P_binding_well_formed Delta Gamma b := 
-    LR_logically_approximate_binding Delta Gamma b b.
+  forall Delta_t Gamma_t bsGn t t' T bs bs',
+    Delta_t = mupdate Delta (binds_Delta b) ->
+    map_normalise (binds_Gamma b) bsGn ->
+    Gamma_t = mupdate Gamma bsGn ->
+    LR_logically_approximate Delta_t Gamma_t (Let NonRec bs t) (Let NonRec bs' t') T ->
+    LR_logically_approximate Delta Gamma (Let NonRec (b :: bs) t) (Let NonRec (b :: bs') t') T.
 
 #[export] Hint Unfold 
   P_has_type
